---
layout: post
title: Curious combinatorial identity
date: 2020-04-20 11:12:00-0400
description: First math post
tags: math science
categories: idea
hidden: true
---


It is often the case in mathematics, when seemingly unrelated ideas suddenly exhibit curious connections. That's precisely where beauty lies. Let me share with you a combinatorial identity that recently was presented to me.
{: .text-justify}

For all intergers $$n \geq 0$$, it follows
{: .text-justify}

$$ \displaystyle \sum_{k=0}^{n}\dbinom{n-k}{k} = F_{n+1} $$.
{: style="font-size: 120%; text-align: center;"}

where $$ F_{n+1}$$ corresponds to the $$(n+1)^{th}$$ term of the [Fibonacci sequence](http://oeis.org/A000045), and the combinatorial number $$ \displaystyle \dbinom{n}{k} = \frac{n!}{k!(n-k)!} $$ is assumed to be zero for $$ n < k $$.
{: .text-justify}


### Proof

We prove the identity using strong induction. For the base case, we trivially verify $$\binom{0}{0} = F_1 = 1$$. 

As inductive step, we assume that the identity holds for all integers $$n'$$ such that $$ 0 \leq n' \leq n $$. Then, we want to deduce that our hypothesis implies the identity holds for $$ n' = n + 1 $$. That is, 

$$ \displaystyle \sum_{k=0}^{n+1}\dbinom{n+1-k}{k} = \dbinom{n+1}{0} + \dbinom{n}{1} + \cdots + \dbinom{0}{n+1} = F_{n+2}$$.
{: style="font-size: 100%; text-align: center;"}

We need to consider the "Pascal's Triangle" formula for combinatorials,

$$ \displaystyle \dbinom{n}{k} = \dbinom{n-1}{k} + \dbinom{n-1}{k-1} $$.
{: style="font-size: 100%; text-align: center;"}

Thus, by applying this formula to all terms except the first and last ones,

$$ \displaystyle \sum_{k=0}^{n+1}\dbinom{n+1-k}{k} = \dbinom{n+1}{0} + \dbinom{n}{1} + \cdots + \dbinom{0}{n+1} $$.

$$ \displaystyle \sum_{k=0}^{n+1}\dbinom{n+1-k}{k} = \dbinom{n+1}{0} + \left( \dbinom{n-1}{1} + \dbinom{n-1}{0} \right)  + \cdots + \dbinom{0}{n+1} $$.

$$ \displaystyle \sum_{k=0}^{n+1}\dbinom{n+1-k}{k} = \dbinom{n}{0} + \left( \dbinom{n-1}{1} + \dbinom{n-1}{0} \right)  + \cdots + \dbinom{0}{n} $$.

$$ \displaystyle \sum_{k=0}^{n+1}\dbinom{n+1-k}{k} = F_{n+1} + F_{n} = F_{n+2} $$.

Therefore, we proved the identity holds for all integers $$ n \geq 0 $$. âˆŽ
